Core/Metatheory/Rename.lean
@@ -17,7 +17,7 @@ theorem subst_lift [RenMap T] (σ : Subst T) :
   rw [ih]
 
 theorem Kinding.closed_rep :
-  G;Δ ⊢ A : K ->
+  G&Δ ⊢ A : K ->
   ∀ (σ : Subst Ty), A[rep Subst.lift σ Δ.length:_] = A
 := by
   intro j; induction j <;> intro σ <;> simp
@@ -34,22 +34,78 @@ theorem Kinding.closed_rep :
   case eq ih1 ih2 =>
     rw [ih1 σ, ih2 σ]; simp
 
-theorem Kinding.closed : G;[] ⊢ A : K -> ∀ σ, A[σ] = A := by
+theorem Kinding.closed : G&[] ⊢ A : K -> ∀ σ, A[σ] = A := by
   intro j; apply closed_rep j
 
--- theorem GlobalWf.closed {G : List Global} :
---   GlobalWf G g ->
---   some T = g.type ->
---   ∀ σ, T[σ] = T
--- := by
---   intro j h
---   induction G
---   sorry
+theorem GlobalWf.head {G : List Global} : ⊢ (g :: G) -> GlobalWf G g := by
+  intro j; cases j; case _ j => exact j
+
+theorem GlobalWf.tail {G : List Global} : ⊢ (g :: G) -> ⊢ G := by
+  intro j; cases j; case _ j _ => exact j
+
+theorem GlobalWf.closed_ctors :
+  ((Option.map Entry.type d).get! = some T -> ∀ σ, T[σ] = T) ->
+  (∀ i e, v i = some e -> e.type = some T -> ∀ σ, T[σ] = T) ->
+  (Option.map Entry.type (Vec.fold Option.or d v)).get! = some T ->
+  ∀ σ, T[σ] = T
+:= by
+  intro h1 h2 h3
+  induction v using Vec.induction <;> simp at h3
+  case nc => apply h1 h3
+  case cc t v ih =>
+    cases t <;> simp at h3
+    case _ =>
+      apply ih _ h3
+      intro i en e1 e2
+      replace h2 := h2 (Fin.succ i) en (by simp; exact e1) e2
+      apply h2
+    case _ en =>
+      apply h2 0 _ _ h3; simp
+
+theorem GlobalWf.closed {G : List Global} :
+  ⊢ G ->
+  lookup_type G x = some T ->
+  ∀ σ, T[σ] = T
+:= by
+  intro j h
+  unfold lookup_type at h
+  fun_induction lookup
+  all_goals try solve | simp [Entry.type] at h
+  all_goals try solve | case _ ih => apply ih (tail j) h
+  case _ n y K cs1 tl cs2 e ih =>
+    have lem := head j
+    cases lem; case _ ctors =>
+    apply closed_ctors (ih (tail j)) _ h
+    intro i e q1 q2
+    subst cs2; simp at q1; rcases q1 with ⟨e1, e2⟩
+    generalize zdef : cs1 i = z at *
+    rcases z with ⟨y, T'⟩; simp at *; subst e1 e2
+    simp [Entry.type] at q2; subst q2
+    replace ctors := ctors i x T' (by rw [zdef])
+    apply Kinding.closed ctors.1
+  case _ y T tl e =>
+    replace e := LawfulBEq.eq_of_beq e
+    simp [Entry.type] at h; subst e h
+    have lem := head j
+    cases lem ; case _ j =>
+    apply Kinding.closed j
+  case _ y T b tl e =>
+    replace e := LawfulBEq.eq_of_beq e
+    simp [Entry.type] at h; subst e h
+    have lem := head j
+    cases lem; case _ j1 j2 =>
+    apply Kinding.closed j1
+  case _ y T tl e =>
+    replace e := LawfulBEq.eq_of_beq e
+    simp [Entry.type] at h; subst e h
+    have lem := head j
+    cases lem; case _ j =>
+    apply Kinding.closed j
 
 theorem Kinding.rename Δr (r : Ren) :
   (∀ i, Δ[i]? = Δr[r i]?) ->
-  G;Δ ⊢ A : K ->
-  G;Δr ⊢ A[r] : K
+  G&Δ ⊢ A : K ->
+  G&Δr ⊢ A[r] : K
 := by
   intro h j
   induction j generalizing Δr r <;> simp
@@ -68,25 +124,67 @@ theorem Kinding.rename Δr (r : Ren) :
   case app ih1 ih2 => apply Kinding.app (ih1 _ _ h) (ih2 _ _ h)
   case eq ih1 ih2 => apply Kinding.eq (ih1 _ _ h) (ih2 _ _ h)
 
-theorem Kinding.weaken : G;Δ ⊢ A : K -> G;(T::Δ) ⊢ A[+1] : K := by
+theorem Kinding.weaken : G&Δ ⊢ A : K -> G&(T::Δ) ⊢ A[+1] : K := by
   intro j; apply rename (T::Δ) (· + 1) _ j
   intro i; cases i <;> simp
 
-theorem Typing.rename_type Δr (r : Ren) :
-  (∀ i, Δ[i]? = Δr[r i]?) ->
-  G;Δ,Γ ⊢ t : A ->
-  G;Δr,Γ.map (·[r]) ⊢ t[r:Ty] : A[r]
+theorem ValidHeadVariable.rename [RenMap T] [SubstMap Term T] (r : Ren)
+  : ValidHeadVariable t test -> ValidHeadVariable t[r:T] test
 := by
-  intro h j; induction j generalizing Δr r <;> simp
+  intro j; cases j; case _ u e =>
+  rcases u with ⟨x, sp⟩
+  rcases e with ⟨e1, e2⟩; simp at e2
+  apply Exists.intro (x, _); rw [e2]; simp
+  have lem := Spine.apply_eq e1
+  rw [lem]
+  sorry; sorry
+
+theorem ValidTyHeadVariable.rename (r : Ren) :
+  ValidTyHeadVariable t test -> ValidTyHeadVariable t[r] test
+:= by
+  sorry
+
+theorem StableTypeMatch.rename Δr (r : Ren) :
+  (∀ i, Δ[i]? = Δr[r i]?) ->
+  StableTypeMatch Δ A B ->
+  StableTypeMatch Δr A[r] B[r]
+:= by
+  sorry
+
+theorem PrefixTypeMatch.rename Δr (r : Ren) :
+  (∀ i, Δ[i]? = Δr[r i]?) ->
+  PrefixTypeMatch Δ A B C ->
+  PrefixTypeMatch Δr A[r] B[r] C[r]
+:= by
+  sorry
+
+theorem Typing.rename_type Δr (r : Ren) :
+  ⊢ G ->
+  (∀ i, Δ[i]? = Δr[r i]?) ->
+  G&Δ,Γ ⊢ t : A ->
+  G&Δr,Γ.map (·[r]) ⊢ t[r:Ty] : A[r]
+:= by
+  intro wf h j; induction j generalizing Δr r <;> simp
   case var j1 j2 =>
     apply Typing.var
     simp; apply Exists.intro _
     apply And.intro j1 rfl
     apply Kinding.rename _ r h j2
   case global j1 j2 =>
-    sorry
+    rw [GlobalWf.closed wf j1]
+    replace j2 := Kinding.rename Δr r h j2
+    rw [GlobalWf.closed wf j1] at j2
+    apply Typing.global j1 j2
   case mtch => sorry
-  case guard => sorry
+  case guard j1 j2 j3 j4 j5 j6 j7 ih1 ih2 ih3 =>
+    apply Typing.guard
+    apply ih1 _ _ h
+    apply ih2 _ _ h
+    apply ih3 _ _ h
+    apply ValidHeadVariable.rename r j4
+    apply ValidTyHeadVariable.rename r j5
+    apply StableTypeMatch.rename _ _ h j6
+    apply PrefixTypeMatch.rename _ _ h j7
   case lam => sorry
   case app => sorry
   case lamt => sorry
@@ -103,3 +201,40 @@ theorem Typing.rename_type Δr (r : Ren) :
   case apptc => sorry
   case zero => sorry
   case choice => sorry
+
+theorem Typing.rename Γr (r : Ren) :
+  ⊢ G ->
+  (∀ {i A}, Γ[i]? = some A -> Γr[r i]? = some A) ->
+  G&Δ,Γ ⊢ t : A ->
+  G&Δ,Γr ⊢ t[r] : A
+:= by
+  intro wf h j; induction j generalizing Γr r <;> simp
+  case var j1 j2 => simp [Ren.to]; apply Typing.var (h j1) j2
+  case global j1 j2 => apply Typing.global j1 j2
+  case mtch => sorry
+  case guard j1 j2 j3 j4 j5 j6 j7 ih1 ih2 ih3 =>
+    apply Typing.guard
+    apply ih1 _ _ h
+    apply ih2 _ _ h
+    apply ih3 _ _ h
+    apply ValidHeadVariable.rename r j4
+    apply j5; apply j6; apply j7
+  case lam => sorry
+  case app => sorry
+  case lamt => sorry
+  case appt => sorry
+  case cast => sorry
+  case refl => sorry
+  case sym => sorry
+  case seq => sorry
+  case appc => sorry
+  case arrowc => sorry
+  case fst => sorry
+  case snd => sorry
+  case allc => sorry
+  case apptc => sorry
+  case zero => sorry
+  case choice => sorry
+
+theorem Typing.weaken T : ⊢ G -> G&Δ,Γ ⊢ t : A -> G&Δ,(T::Γ) ⊢ t[+1] : A := by
+  intro wf j; apply rename (T::Γ) (· + 1) wf _ j; simp
