Core/Term.lean
@@ -1,4 +1,5 @@
 import Core.Term.Definition
+import Core.Term.BEq
 import Core.Term.Substitution
 import Core.Term.Spine
 import Core.Term.Variant
